examples/wysteria/mill3.fst
@@ -1,5 +1,5 @@
 (*--build-config
-    options:--admit_fsi Set --admit_fsi Wysteria;
+    options:--admit_fsi Set --admit_fsi Wysteria --codegen Wysteria;
     variables:LIB=../../lib;
     other-files:$LIB/ghost.fst $LIB/ext.fst $LIB/set.fsi $LIB/heap.fst $LIB/st.fst $LIB/all.fst wysteria.fsi
  --*)
@@ -20,8 +20,13 @@ let abc = union ab charlie_s
 type pre  (m:mode)  = fun m0 -> b2t (m0 = m)
 type post (#a:Type) = fun (m:mode) (x:a) -> True
 
+val read_fn: unit -> Wys nat (fun m0 -> Mode.m m0 = Par /\
+                                        (exists p. Mode.ps m0 = singleton p))
+                             (fun m0 r -> True)
+let read_fn x = read #nat ()
+
 val mill3_sec: #p1:prin -> #p2:prin
-               -> x:Box nat (singleton p1) -> y:Box nat (singleton p2)
+               -> x:Box int (singleton p1) -> y:Box int (singleton p2)
                -> unit
                -> Wys bool (pre (Mode Par (union (singleton p1) (singleton p2)))) post
 let mill3_sec #p1 #p2 x y _ =
@@ -31,16 +36,17 @@ let mill3_sec #p1 #p2 x y _ =
   in
   as_sec s g
 
-val mill3: unit -> Wys bool (pre (Mode Par abc)) post
+val mill3: unit -> Wys (Box bool bc) (pre (Mode Par abc)) post
 let mill3 _ =
-  let x = as_par alice_s (read #nat) in
-  let y = as_par bob_s (read #nat) in
-  let z = as_par charlie_s (read #nat) in
+  let x = as_par alice_s read_fn in
+  let y = as_par bob_s read_fn in
+  let z = as_par charlie_s read_fn in
 
-  let _ = as_par ab (mill3_sec #alice #bob x y) in
-  let _ = as_par bc (mill3_sec #bob #charlie y z) in
+  let p = as_par ab (mill3_sec #alice #bob x y) in
+  let q = as_par bc (mill3_sec #bob #charlie y z) in
 
-  true
+  q
 ;;
 
-let _ = main abc mill3 in ()
+let q = main abc mill3 in
+wprint ()
